Fomega/Ctx.lean
@@ -1,0 +1,22 @@
+
+import Common
+
+namespace Fomega
+
+  abbrev Ctx := List Term
+
+  namespace Ctx
+
+    def apply : Subst Term -> Ctx -> Ctx
+    | _, [] => []
+    | σ, .cons h t => .cons ([σ]h) (apply ^σ t)
+
+    def beta : Ctx -> Term -> Ctx
+    | s, t => apply ((.replace t) :: (r#I)) s
+
+  end Ctx
+
+end Fomega
+
+notation:90 "[" σ "]" t:89 => Fomega.Ctx.apply σ t
+notation:90 s:90 "β[" t "]" => Fomega.Ctx.beta s t
