Fomega/Proof.lean
@@ -1,0 +1,51 @@
+
+import Common
+import Fomega.Ctx
+
+namespace Fomega
+
+  inductive Conv : Term -> Term -> Prop
+  | ax : Conv ★ ★
+  | bound x : Conv (.bound K x) (.bound K x)
+  | all_congr : Conv A1 A2 -> Conv B1 B2 -> Conv (.all mf A1 B1) (.all mf A2 B2)
+  | lam_congr : Conv A1 A2 -> Conv t1 t2 -> Conv (.lam mf A1 t1) (.lam mf A2 t2)
+  | lam_eta : Conv (.lam mf A t1) (Term.eta mf A t2) -> Conv (.lam mf A t1) t2
+  | app_congr : Conv f1 f2 -> Conv a1 a2 -> Conv (.app m f1 a1) (.app m f2 a2)
+  | app_beta : Conv (b β[t]) t2 -> Conv (.app mf (.lam mf A b) t) t2
+
+end Fomega
+
+notation:100 A:32 " === " B:31 => Fomega.Conv A B
+
+namespace Fomega
+
+  inductive Proof : Ctx -> Term -> Term -> Prop
+  | ax : Proof Γ ★ □
+  | var :
+    Γ = Γ1 ++ [A] ++ Γ2 ->
+    Proof Γ1 A (.const K) ->
+    Proof Γ (.bound K Γ1.length) A
+  | pi :
+    Proof Γ A K ->
+    Proof (Γ ++ [A]) B ★ ->
+    Proof Γ (.all mf A B) ★
+  | tpi :
+    Proof Γ A □ ->
+    Proof (Γ ++ [A]) B □ ->
+    Proof Γ (.all mf A B) □
+  | lam :
+    Proof Γ (.all mf A B) K ->
+    Proof (Γ ++ [A]) t B ->
+    Proof Γ (.lam mf A t) (.all mf A B)
+  | app :
+    Proof Γ f (.all mf A B) ->
+    Proof Γ a A ->
+    Proof Γ (.app mf f a) (B β[a])
+  | conv :
+    Proof Γ t A ->
+    Proof Γ B K ->
+    A === B ->
+    Proof Γ t B
+end Fomega
+
+notation:170 Γ:170 " ⊢ " t:170 " : " A:170 => Fomega.Proof Γ t A
