Fomega/Substitution.lean
@@ -1,0 +1,35 @@
+
+import Common
+import Fomega.Ctx
+import Fomega.Proof
+
+namespace Fomega
+
+  theorem weaken :
+    Γ ⊢ t : A ->
+    let (m, n) := (Δ1.length, Δ2.length)
+    (Δ1 ++ [r#(Sn m)]Γ ++ Δ2) ⊢ ([r#(Sn n)]t) : ([r#(Sn n)]A)
+  := by {
+    sorry
+  }
+
+  theorem proof_subst :
+    Γ1 ⊢ a : A ->
+    (Γ1 ++ [A] ++ Γ2) ⊢ t : T ->
+    let n := Γ2.length
+    (Γ1 ++ ([beta a]Γ2)) ⊢ ([^{n}beta a]t) : ([^{n}beta a]T)
+  := by {
+    intro h j
+    generalize Γdef : Γ1 ++ [A] ++ Γ2 = Γ at j
+    induction j
+    case ax Δ => simp; constructor
+    case var Δ Δ1 T Δ2 K j1 j2 ih =>
+      sorry
+    case pi => sorry
+    case tpi => sorry
+    case lam => sorry
+    case app => sorry
+    case conv => sorry
+  }
+
+end Fomega
